% file: parts/recurrences.tex

%%%%%%%%%%%%%%%
\begin{frame}{}
  \centerline{\teal{\Large Recurrences}}
  \fignocaption{width = 0.60\textwidth}{figs/fractal-tree}
\end{frame}
%%%%%%%%%%%%%%%

%%%%%%%%%%%%%%%
\begin{frame}{}
  \[
    T(n) = aT(n/b) + f(n) \quad (a > 0, b > 1) 
  \]

  \pause
  \centerline{\red{Assume that $T(n)$ is constant for sufficiently small $n$.}}

  \pause
  \vspace{0.30cm}
  \begin{equation*}
    \left.\begin{aligned}
      f(n) \\
      af(\frac{n}{b}) \\
      a^2f(\frac{n}{b^2}) \\
      \vdots \\
      a^{\log_b n} f(\purple{c}) = \Theta(n^{\log_b a})
    \end{aligned}\right\}
    \pause
    \red{\sum}\;\; \blue{\overset{f(n) \text{ vs. } n^{E}}{=}} \left\{\begin{aligned}
      n^{\log_b a}		 \\
      n^{\log_b a}\log n 	 \\
      f(n)		   \quad \\
    \end{aligned}\right.
    \; \left.\begin{aligned}
      f(n) &= O(n^{E-\epsilon}) \\
      f(n) &= \Theta(n^E) \\
      f(n) &= \Omega(n^{E+\epsilon}) 
    \end{aligned}\right.
  \end{equation*}
\end{frame}
%%%%%%%%%%%%%%%

%%%%%%%%%%%%%%%
\begin{frame}{}
  \begin{columns}
    \column{0.30\textwidth}
      \begin{exampleblock}{Solving Recurrences (Problem $2.15$)}
	\begin{enumerate}[(1)]
	  \item $\Theta(n^{\log_3 2})$
	  \item \textcolor{red}{$\Theta(\log^2 n)$}
	  \item $\Theta(n)$
	  \item $\Theta(n \log n)$
	  \item \textcolor{red}{$\Theta(n \log^2 n)$}
	  \item $\Theta(n^2)$
	  \item $\Theta(n^{\frac{3}{2}}\log n)$
	  \item $\Theta(n)$
	  \item \teal{$\Theta(n^{c+1})$}
	  \item \teal{$\Theta(c^{n+1})$}
	  \item \purple{$\cdots$}
	\end{enumerate}
      \end{exampleblock}
    \column{0.65\textwidth}
      \[
	T(n) = T(n/2) + \log n
      \]
      \[
	T(n) = 2T(n/2) + n\log n
      \]

    \pause
    \begin{alertblock}{Reference:}
      \vspace{-0.30cm}
      \[
	f(n) = \Theta(n^{\log_b a} \log^{\red{k}}n) \implies \Theta(n^{\log_b a} \log^{\red{k+1}}n)
      \]
    \end{alertblock}

    \pause
    \[
      T(n) = T(n-1) + n^c \quad c \ge 1
    \]
    \[
      T(n) = T(n-1) + c^n \quad c > 1
    \]
  \end{columns}
\end{frame}
%%%%%%%%%%%%%%%

%%%%%%%%%%%%%%%
\begin{frame}{}
  \begin{exampleblock}{Solving Recurrences (Problem $2.15\; (11)$)}
    \[
      T(n) = T(n/2) + T(n/4) + T(n/8) \pause \;\red{+\; n}
    \]
  \end{exampleblock}

  \pause
  \vspace{0.30cm}
  \centerline{By recursion-tree.}
  \[
    \boxed{\teal{T(n) = \Theta(n)}}
  \]

  \pause
  \vspace{0.50cm}
  \centerline{\red{Exercise: Prove it by mathematical induction.}}

  \pause
  \begin{alertblock}{Reference:}
    {\it ``On the Solution of Linear Recurrence Equations''} by Akra \& Bazzi, 1996.

    \[
      T(n) = \sum_{i=1}^{k} a_i T(n/b_i) + f(n)
    \]
  \end{alertblock}
\end{frame}
%%%%%%%%%%%%%%%

%%%%%%%%%%%%%%%
% \begin{frame}{Gaps (Problem 1.2.16)}
%   \[
%     T(n) = 2T(n/2) + \frac{n}{\log n} \pause = \Theta(n \log \log n)
%   \]
% 
%   \pause
% 
%   The regularity condition in Case 3:
%   \[
% 	bf(n/c) \le cf(n), \text{ for some } c < 1 \text{ and sufficiently large } n
%   \]
% 
%   \[
% 	T(n) = T(n/2) + n(2 - \cos n)
%   \]
% 
%   \[
% 	n^{E} = n^0 \quad f(n) = n(2 - \cos n) = \Omega(n^{0 + \epsilon})
%   \]
% 
%   \pause
%   \[
% 	n = 2\pi k (k \text{ odd}) \Rightarrow c \ge \frac{3}{2}
%   \]
% \end{frame}
%%%%%%%%%%%%%%%

%%%%%%%%%%%%%%%
\begin{frame}{}
  \begin{exampleblock}{Solving Recurrences (Problem $2.17$)}
    \begin{align*} 
      \text{T}(n) &= \sqrt{n}\ \text{T}(\sqrt{n})+n \\
	&= \teal{n^{\frac{1}{2}}\ \text{T}\left(n^{\frac{1}{2}} \right)+n} \\
	&= n^{\frac{1}{2}}\left( n^{\frac{1}{2^2}}\ \text{T}\left(n^{\frac{1}{2^2}} \right) + n^{\frac{1}{2}} \right)+n\\
	&= \teal{n^{\frac{1}{2}+\frac{1}{2^2}}\ \text{T}\left(n^{\frac{1}{2^2}}\right) + 2n} \\
	&= n^{\frac{1}{2}+\frac{1}{2^2}}\left(n^{\frac{1}{2^3}}\ \text{T}\left(n^{\frac{1}{2^3}}\right) + n^{\frac{1}{2^2}} \right) + 2n\\
	&= \teal{n^{\frac{1}{2}+\frac{1}{2^2}+\frac{1}{2^3}}\ \text{T}\left(n^{\frac{1}{2^3}}\right) + 3n} \\ 
	&= \cdots \\ 
	&= \red{n^{\sum_{i=1}^{k}\frac{1}{2^i}}\ \text{T}\left(n^{\frac{1}{2^k}}\right) + kn} \\ 
    \end{align*}
  \end{exampleblock}
\end{frame}
%%%%%%%%%%%%%%%

%%%%%%%%%%%%%%%
\begin{frame}{}
  \[
    n^{\frac{1}{2^k}} = \red{2} \pause \implies k = \log\log n
  \]

  \pause
  \begin{align*} 
    \text{T}(n) &= n^{\sum_{i=1}^{k}\frac{1}{2^i}}\ \text{T}\left(n^{\frac{1}{2^k}}\right ) +kn\\ 
	    &=n^{\sum_{i=1}^{\log\log n}\frac{1}{2^i}}\ \text{T}(2) + n \log\log n\\ 
  \end{align*}

  \pause
  \[
    \sum_{i=1}^{\log_2\log_2(n)}\frac{1}{2^i} < 1 \implies T(n) = \Theta(n \log \log n)
  \]

  \pause
  \vspace{0.30cm}
  \centerline{\red{Exercise: Prove it by mathematical induction.}}
\end{frame}
%%%%%%%%%%%%%%%

%%%%%%%%%%%%%%%
\begin{frame}{}
  \[
    \boxed{T(n) = \sqrt{n} T(\sqrt{n}) + n}
  \]

  \pause
  \[
    \frac{T(n)}{n} = \frac{T(\sqrt{n})}{\sqrt{n}} + 1
  \]

  \pause
  \[
    \red{n \leftrightarrow 2^m}
  \]

  \pause
  \[
    \frac{T(2^m)}{2^m} = \frac{T(2^{m/2})}{2^{m/2}} + 1
  \]

  \pause
  \[
    \red{S(m) \leftrightarrow \frac{T(2^m)}{2^m}}
  \]

  \pause
  \[
    S(m) = S(m/2) + 1 = \pause \Theta(\log m)
  \]

  \pause
  \vspace{-0.60cm}
  \[
    \teal{T(n) = n \log \log n}
  \]
\end{frame}
%%%%%%%%%%%%%%%
