\section{Recurrences}

\begin{frame}{Recurrences}
  \[
	T(n) = aT(n/b) + f(n) \quad (a > 0, b > 1)
  \]

  \begin{equation*}
	\left.\begin{aligned}
	  f(n) \\
	  af(\frac{n}{b}) \\
	  a^2f(\frac{n}{b^2}) \\
	  \vdots \\
	  a^{\log_b^n}f(1) = n^{\log_b^a}
	\end{aligned}\right\}
	\pause
	\sum = \left\{\begin{aligned}
	  n^{\log_b^a}	\quad & q > 1 \\
	  n^{\log_b^a}\log n \quad & q = 1 \\
	  f(n)	\quad & q < 1 \quad \\
	\end{aligned}\right.
	\pause
	\quad \left.\begin{aligned}
	  f(n) &= O(n^{E-\epsilon}) \\
      f(n) &= \Theta(n^E) \\
      f(n) &= \Omega(n^{E+\epsilon}) 
	\end{aligned}\right.
  \end{equation*}
\end{frame}
%%%%%%%%%%%%%%%%%%%%
\begin{frame}{Solving recurrences (Problem 1.2.13, 1.2.16)}
  \begin{columns}
	\column{0.40\textwidth}
	  \begin{enumerate}
		\item $\Theta(n^{\log_3^2})$
		\item \textcolor{red}{$\Theta(\log^2 n)$}
		\item $\Theta(n)$
		\item $\Theta(n \log n)$
		\item \textcolor{red}{$\Theta(n \log^2 n)$}
		\item $\Theta(n^2)$
		\item $\Theta(n^{\frac{3}{2}}\log n)$
		\item $\Theta(n)$
		\item $\Theta(n^{c+1})$
		\item $\Theta(c^{n+1})$
		\item \textcolor{blue}{$\Theta(n)$}
	  \end{enumerate}
	\column{0.60\textwidth}
	  \[
		T(n) = T(n/2) + \log n
	  \]

	  \[
		T(n) = 2T(n/2) + n\log n
	  \]

	\pause
	\begin{alertblock}{Reference}
	  \[
		f(n) = \Theta(n^{\log_b^a} \lg^{k}n) \Rightarrow \Theta(n^{\log_b^a} \lg^{k+1}n)
	  \]
	\end{alertblock}
  \end{columns}
\end{frame}
%%%%%%%%%%%%%%%%%%%%
\begin{frame}{Solving recurrences (Problem 1.2.13, 1.2.16)}
  \[
	T(n) = T(n/2) + T(n/4) + T(n/8) + n
  \]

  \pause
  \vspace{0.30cm}
  \centerline{By recursion-tree.}

  \pause
  \vspace{0.50cm}
  
  \centerline{Exercise: Prove it by Mathematical Induction.}

  \pause
  \begin{alertblock}{Reference}
	``On the Solution of Linear Recurrence Equations'' by Akra \& Bazzi, 1996.

	\[
	  T(n) = \sum_{i=1}^{k} a_i T(n/b_i) + f(n)
	\]
  \end{alertblock}
\end{frame}
%%%%%%%%%%%%%%%%%%%%
\begin{frame}{Gaps (Problem 1.2.16)}
  \[
	T(n) = 2T(n/2) + \frac{n}{\log n} \pause = \Theta(n \log \log n)
  \]

  \pause

  The regularity condition in Case 3:
  \[
	bf(n/c) \le cf(n), \text{ for some } c < 1 \text{ and sufficiently large } n
  \]

  \[
	T(n) = T(n/2) + n(2 - \cos n)
  \]

  \[
	n^{E} = n^0 \quad f(n) = n(2 - \cos n) = \Omega(n^{0 + \epsilon})
  \]

  \pause
  \[
	n = 2\pi k (k \text{ odd}) \Rightarrow c \ge \frac{3}{2}
  \]
\end{frame}
%%%%%%%%%%%%%%%%%%%%
\begin{frame}{(Problem 1.2.15)}
  \begin{align*} 
	\text{T}(n) &= \sqrt{n}\ \text{T}(\sqrt{n})+n \\
		&= n^{\frac{1}{2}}\ \text{T}\left(n^{\frac{1}{2}} \right )+n \\
		&= n^{\frac{1}{2}}\left( n^{\frac{1}{2^2}}\ \text{T}\left(n^{\frac{1}{2^2}} \right )+n^{\frac{1}{2}} \right )+n\\
		&= n^{\frac{1}{2}+\frac{1}{2^2}}\ \text{T}\left(n^{\frac{1}{2^2}}\right ) +2n\\
		&= n^{\frac{1}{2}+\frac{1}{2^2}}\left(n^{\frac{1}{2^3}}\ \text{T}\left(n^{\frac{1}{2^3}}\right ) +n^{\frac{1}{2^2}} \right )+2n\\
		&= n^{\frac{1}{2}+\frac{1}{2^2}+\frac{1}{2^3}}\ \text{T}\left(n^{\frac{1}{2^3}}\right ) +3n\\ 
		&= \cdots \\ 
		&= n^{\sum_{i=1}^{k}\frac{1}{2^i}}\ \text{T}\left(n^{\frac{1}{2^k}}\right ) +kn\\ 
  \end{align*}
\end{frame}
%%%%%%%%%%%%%%%%%%%%
\begin{frame}{(Problem 1.2.15)}
  \[
	n^{\frac{1}{2^k}} = 2 \Rightarrow k = \log\log n
  \]

  \pause

  \begin{align*} 
	\text{T}(n) &= n^{\sum_{i=1}^{k}\frac{1}{2^i}}\ \text{T}\left(n^{\frac{1}{2^k}}\right ) +kn\\ 
		&=n^{\sum_{i=1}^{\log\log n}\frac{1}{2^i}}\ \text{T}(2) + n \log\log n\\ 
  \end{align*}

  \pause
  \[
	\sum_{i=1}^{\log_2\log_2(n)}\frac{1}{2^i} < 1 \Rightarrow T(n) = \Theta(n \log \log n)
  \]

  \pause
  \vspace{0.30cm}
  \centerline{Exercise: Prove it by Mathematical Induction.}
\end{frame}
%%%%%%%%%%%%%%%%%%%%
\begin{frame}{(Problem 1.2.15)}
  \[
	T(n) = \sqrt{n} T(\sqrt{n}) + n
  \]

  \[
	n = 2^k \quad \sqrt{n} = 2^{k/2} \quad k = \log n
  \]
\end{frame}
%%%%%%%%%%%%%%%%%%%%
%%%%%%%%%%%%%%%%%%%%
%%%%%%%%%%%%%%%%%%%%
